Generalize equality of heap_lang so it works on any value.
This is more consistent with CAS, which also can be used on any value.
Note that being able to (atomically) test for equality of any value and
being able to CAS on any value is not realistic. See the discussion at
https://gitlab.mpi-sws.org/FP/iris-coq/issues/26, and in particular JH
Jourdan's observation:

  I think indeed for heap_lang this is just too complicated.

  Anyway, the role of heap_lang is not to model any actual
  programming language, but rather to show that we can do proofs
  about certain programs. The fact that you can write unrealistic
  programs is not a problem, IMHO. The only thing which is important
  is that the program that we write are realistic (i.e., faithfully
  represents the algorithm we want to p

This commit is based on a commit by Zhen Zhang who generalized equality
to work on any literal (and not just integers).

heap_lang/lang.v
@@ -133,6 +133,40 @@ Fixpoint to_val (e : expr) : option val :=
 (** The state: heaps of vals. *)
 Definition state := gmap loc val.
 
+(** Equality and other typeclass stuff *)
+Lemma to_of_val v : to_val (of_val v) = Some v.
+Proof.
+  by induction v; simplify_option_eq; repeat f_equal; try apply (proof_irrel _).
+Qed.
+
+Lemma of_to_val e v : to_val e = Some v → of_val v = e.
+Proof.
+  revert v; induction e; intros v ?; simplify_option_eq; auto with f_equal.
+Qed.
+
+Instance of_val_inj : Inj (=) (=) of_val.
+Proof. by intros ?? Hv; apply (inj Some); rewrite -!to_of_val Hv. Qed.
+
+Instance base_lit_dec_eq (l1 l2 : base_lit) : Decision (l1 = l2).
+Proof. solve_decision. Defined.
+Instance un_op_dec_eq (op1 op2 : un_op) : Decision (op1 = op2).
+Proof. solve_decision. Defined.
+Instance bin_op_dec_eq (op1 op2 : bin_op) : Decision (op1 = op2).
+Proof. solve_decision. Defined.
+Instance expr_dec_eq (e1 e2 : expr) : Decision (e1 = e2).
+Proof. solve_decision. Defined.
+Instance val_dec_eq (v1 v2 : val) : Decision (v1 = v2).
+Proof.
+ refine (cast_if (decide (of_val v1 = of_val v2))); abstract naive_solver.
+Defined.
+
+Instance expr_inhabited : Inhabited expr := populate (Lit LitUnit).
+Instance val_inhabited : Inhabited val := populate (LitV LitUnit).
+
+Canonical Structure stateC := leibnizC state.
+Canonical Structure valC := leibnizC val.
+Canonical Structure exprC := leibnizC expr.
+
 (** Evaluation contexts *)
 Inductive ectx_item :=
   | AppLCtx (e2 : expr)
@@ -208,20 +242,20 @@ Definition subst' (mx : binder) (es : expr) : expr → expr :=
   match mx with BNamed x => subst x es | BAnon => id end.
 
 (** The stepping relation *)
-Definition un_op_eval (op : un_op) (l : base_lit) : option base_lit :=
-  match op, l with
-  | NegOp, LitBool b => Some (LitBool (negb b))
-  | MinusUnOp, LitInt n => Some (LitInt (- n))
+Definition un_op_eval (op : un_op) (v : val) : option val :=
+  match op, v with
+  | NegOp, LitV (LitBool b) => Some $ LitV $ LitBool (negb b)
+  | MinusUnOp, LitV (LitInt n) => Some $ LitV $ LitInt (- n)
   | _, _ => None
   end.
 
-Definition bin_op_eval (op : bin_op) (l1 l2 : base_lit) : option base_lit :=
-  match op, l1, l2 with
-  | PlusOp, LitInt n1, LitInt n2 => Some $ LitInt (n1 + n2)
-  | MinusOp, LitInt n1, LitInt n2 => Some $ LitInt (n1 - n2)
-  | LeOp, LitInt n1, LitInt n2 => Some $ LitBool $ bool_decide (n1 ≤ n2)
-  | LtOp, LitInt n1, LitInt n2 => Some $ LitBool $ bool_decide (n1 < n2)
-  | EqOp, LitInt n1, LitInt n2 => Some $ LitBool $ bool_decide (n1 = n2)
+Definition bin_op_eval (op : bin_op) (v1 v2 : val) : option val :=
+  match op, v1, v2 with
+  | PlusOp, LitV (LitInt n1), LitV (LitInt n2) => Some $ LitV $ LitInt (n1 + n2)
+  | MinusOp, LitV (LitInt n1), LitV (LitInt n2) => Some $ LitV $ LitInt (n1 - n2)
+  | LeOp, LitV (LitInt n1), LitV (LitInt n2) => Some $ LitV $ LitBool $ bool_decide (n1 ≤ n2)
+  | LtOp, LitV (LitInt n1), LitV (LitInt n2) => Some $ LitV $ LitBool $ bool_decide (n1 < n2)
+  | EqOp, v1, v2 => Some $ LitV $ LitBool $ bool_decide (v1 = v2)
   | _, _, _ => None
   end.
 
@@ -231,12 +265,14 @@ Inductive head_step : expr → state → expr → state → list (expr) → Prop
      Closed (f :b: x :b: []) e1 →
      e' = subst' x (of_val v2) (subst' f (Rec f x e1) e1) →
      head_step (App (Rec f x e1) e2) σ e' σ []
-  | UnOpS op l l' σ :
-     un_op_eval op l = Some l' → 
-     head_step (UnOp op (Lit l)) σ (Lit l') σ []
-  | BinOpS op l1 l2 l' σ :
-     bin_op_eval op l1 l2 = Some l' → 
-     head_step (BinOp op (Lit l1) (Lit l2)) σ (Lit l') σ []
+  | UnOpS op e v v' σ :
+     to_val e = Some v →
+     un_op_eval op v = Some v' → 
+     head_step (UnOp op e) σ (of_val v') σ []
+  | BinOpS op e1 e2 v1 v2 v' σ :
+     to_val e1 = Some v1 → to_val e2 = Some v2 →
+     bin_op_eval op v1 v2 = Some v' → 
+     head_step (BinOp op e1 e2) σ (of_val v') σ []
   | IfTrueS e1 e2 σ :
      head_step (If (Lit $ LitBool true) e1 e2) σ e1 σ []
   | IfFalseS e1 e2 σ :
@@ -274,19 +310,6 @@ Inductive head_step : expr → state → expr → state → list (expr) → Prop
      head_step (CAS (Lit $ LitLoc l) e1 e2) σ (Lit $ LitBool true) (<[l:=v2]>σ) [].
 
 (** Basic properties about the language *)
-Lemma to_of_val v : to_val (of_val v) = Some v.
-Proof.
-  by induction v; simplify_option_eq; repeat f_equal; try apply (proof_irrel _).
-Qed.
-
-Lemma of_to_val e v : to_val e = Some v → of_val v = e.
-Proof.
-  revert v; induction e; intros v ?; simplify_option_eq; auto with f_equal.
-Qed.
-
-Instance of_val_inj : Inj (=) (=) of_val.
-Proof. by intros ?? Hv; apply (inj Some); rewrite -!to_of_val Hv. Qed.
-
 Instance fill_item_inj Ki : Inj (=) (=) (fill_item Ki).
 Proof. destruct Ki; intros ???; simplify_eq/=; auto with f_equal. Qed.
 
@@ -334,27 +357,6 @@ Proof. intros. apply is_closed_subst with []; set_solver. Qed.
 
 Lemma is_closed_of_val X v : is_closed X (of_val v).
 Proof. apply is_closed_weaken_nil. induction v; simpl; auto. Qed.
-
-(** Equality and other typeclass stuff *)
-Instance base_lit_dec_eq (l1 l2 : base_lit) : Decision (l1 = l2).
-Proof. solve_decision. Defined.
-Instance un_op_dec_eq (op1 op2 : un_op) : Decision (op1 = op2).
-Proof. solve_decision. Defined.
-Instance bin_op_dec_eq (op1 op2 : bin_op) : Decision (op1 = op2).
-Proof. solve_decision. Defined.
-Instance expr_dec_eq (e1 e2 : expr) : Decision (e1 = e2).
-Proof. solve_decision. Defined.
-Instance val_dec_eq (v1 v2 : val) : Decision (v1 = v2).
-Proof.
- refine (cast_if (decide (of_val v1 = of_val v2))); abstract naive_solver.
-Defined.
-
-Instance expr_inhabited : Inhabited expr := populate (Lit LitUnit).
-Instance val_inhabited : Inhabited val := populate (LitV LitUnit).
-
-Canonical Structure stateC := leibnizC state.
-Canonical Structure valC := leibnizC val.
-Canonical Structure exprC := leibnizC expr.
 End heap_lang.
 
 (** Language *)
