heap_lang/wp_tactics.v
@@ -88,11 +88,14 @@ Tactic Notation "wp_op" :=
     lazymatch eval hnf in e' with
     | BinOp LtOp _ _ => wp_bind_core K; apply wp_lt; wp_finish
     | BinOp LeOp _ _ => wp_bind_core K; apply wp_le; wp_finish
-    | BinOp EqOp _ _ => wp_bind_core K; apply wp_eq; wp_finish
+    | BinOp EqOp _ _ =>
+       wp_bind_core K; eapply wp_eq; [wp_done|wp_done|wp_finish|wp_finish]
     | BinOp _ _ _ =>
-       wp_bind_core K; etrans; [|eapply wp_bin_op; try fast_done]; wp_finish
+       wp_bind_core K; etrans;
+         [|eapply wp_bin_op; [wp_done|wp_done|try fast_done]]; wp_finish
     | UnOp _ _ =>
-       wp_bind_core K; etrans; [|eapply wp_un_op; try fast_done]; wp_finish
+       wp_bind_core K; etrans;
+         [|eapply wp_un_op; [wp_done|try fast_done]]; wp_finish
     end) || fail "wp_op: cannot find 'BinOp' or 'UnOp' in" e
   | _ => fail "wp_op: not a 'wp'"
   end.
