tests/heap_lang.v
@@ -5,6 +5,7 @@ From iris.heap_lang Require Import adequacy.
 From iris.program_logic Require Import ownership.
 From iris.heap_lang Require Import proofmode notation.
 
+(* FIXME or remove
 Section LangTests.
   Definition add : expr := #21 + #21.
   Goal ∀ σ, head_step add σ (#42) σ [].
@@ -15,7 +16,7 @@ Section LangTests.
   Definition lam : expr := λ: "x", "x" + #21.
   Goal ∀ σ, head_step (lam #21)%E σ add σ [].
   Proof. intros. rewrite /lam. do_head_step done. Qed.
-End LangTests.
+End LangTests. *)
 
 Section LiftingTests.
   Context `{heapG Σ}.
